done

Foundation/Modal/Kripke/Rank.lean
@@ -10,113 +10,113 @@ namespace Kripke
 variable {φ ψ : Formula ℕ}
          {F : Frame} {r : F} [Fintype F] [F.IsTree r] {x y i j : F}
 
-def Frame.World.finHeight (i : F) : ℕ := fcwHeight (· ≺ ·) i
+def Frame.rank (i : F) : ℕ := fcwHeight (· ≺ ·) i
 
-def Frame.finHeight (F : Frame) {r : F} [Fintype F] [F.IsTree r] : ℕ := Frame.World.finHeight r
+def Frame.height (F : Frame) {r : F} [Fintype F] [F.IsTree r] : ℕ := Frame.rank r
 
 namespace Frame
 
-lemma World.finHeight_lt_whole_finHeight {i : F} (hi : r ≺ i) :
-    Frame.World.finHeight i < F.finHeight := fcwHeight_gt_of hi
+lemma rank_lt_whole_height {i : F} (hi : r ≺ i) :
+    F.rank i < F.height := fcwHeight_gt_of hi
 
-lemma World.finHeight_le_whole_finHeight (i : F) :
-    Frame.World.finHeight i ≤ F.finHeight := by
+lemma rank_le_whole_height (i : F) :
+    F.rank i ≤ F.height := by
   by_cases hi : i = r
   · rcases hi; rfl
   · have : r ≺ i := root_genaretes'! i hi
     exact le_of_lt (fcwHeight_gt_of this)
 
-lemma World.finHeight_lt_of_rel (hij : i ≺ j) : Frame.World.finHeight i > Frame.World.finHeight j := fcwHeight_gt_of hij
+lemma rank_lt_of_rel (hij : i ≺ j) : F.rank i > Frame.rank j := fcwHeight_gt_of hij
 
-lemma World.exists_of_lt_finHeight (hn : n < Frame.World.finHeight i) : ∃ j : F, i ≺ j ∧ Frame.World.finHeight j = n := fcwHeight_lt hn
+lemma exists_of_lt_height (hn : n < F.rank i) : ∃ j : F, i ≺ j ∧ Frame.rank j = n := fcwHeight_lt hn
 
-lemma finHeight_lt_iff_relItr {i : F} :
-    Frame.World.finHeight i < n ↔ ∀ j, ¬i ≺^[n] j  := by
+lemma height_lt_iff_relItr {i : F} :
+    F.rank i < n ↔ ∀ j, ¬i ≺^[n] j  := by
   match n with
   |     0 => simp_all
   | n + 1 =>
-    suffices Frame.World.finHeight i ≤ n ↔ ∀ j : F, i ≺ j → Frame.World.finHeight j < n by
+    suffices F.rank i ≤ n ↔ ∀ j : F, i ≺ j → Frame.rank j < n by
       calc
-        Frame.World.finHeight i < n + 1
-          ↔ Frame.World.finHeight i ≤ n := Nat.lt_add_one_iff
-        _ ↔ ∀ j, i ≺ j → Frame.World.finHeight j < n := this
-        _ ↔ ∀ j, i ≺ j → ∀ k, ¬j ≺^[n] k := by simp [finHeight_lt_iff_relItr (n := n)]
+        F.rank i < n + 1
+          ↔ F.rank i ≤ n := Nat.lt_add_one_iff
+        _ ↔ ∀ j, i ≺ j → Frame.rank j < n := this
+        _ ↔ ∀ j, i ≺ j → ∀ k, ¬j ≺^[n] k := by simp [height_lt_iff_relItr (n := n)]
         _ ↔ ∀ k j, i ≺ j → ¬j ≺^[n] k    := by grind
         _ ↔ ∀ j, ¬i ≺^[n + 1] j  := by simp
     constructor
     · exact fun h j hij ↦ lt_of_lt_of_le (fcwHeight_gt_of hij) h
     · exact fcwHeight_le
 
-lemma le_finHeight_iff_relItr {i : F} :
-    n ≤ Frame.World.finHeight i ↔ ∃ j, i ≺^[n] j := calc
-  n ≤ Frame.World.finHeight i ↔ ¬Frame.World.finHeight i < n := Iff.symm Nat.not_lt
-  _                           ↔ ∃ j, i ≺^[n] j := by simp [finHeight_lt_iff_relItr]
+lemma le_height_iff_relItr {i : F} :
+    n ≤ F.rank i ↔ ∃ j, i ≺^[n] j := calc
+  n ≤ F.rank i ↔ ¬F.rank i < n := Iff.symm Nat.not_lt
+  _                           ↔ ∃ j, i ≺^[n] j := by simp [height_lt_iff_relItr]
 
-lemma finHeight_eq_iff_relItr {i : F} :
-    Frame.World.finHeight i = n ↔ (∃ j, i ≺^[n] j) ∧ (∀ j, i ≺^[n] j → ∀ k, ¬j ≺ k) := calc
-  Frame.World.finHeight i = n
-    ↔ Frame.World.finHeight i < n + 1 ∧ n ≤ Frame.World.finHeight i := by simpa [Nat.lt_succ_iff] using Nat.eq_iff_le_and_ge
-  _ ↔ (∀ j, ¬i ≺^[n + 1] j) ∧ (∃ j, i ≺^[n] j) := by simp [finHeight_lt_iff_relItr, le_finHeight_iff_relItr]
+lemma height_eq_iff_relItr {i : F} :
+    F.rank i = n ↔ (∃ j, i ≺^[n] j) ∧ (∀ j, i ≺^[n] j → ∀ k, ¬j ≺ k) := calc
+  F.rank i = n
+    ↔ F.rank i < n + 1 ∧ n ≤ F.rank i := by simpa [Nat.lt_succ_iff] using Nat.eq_iff_le_and_ge
+  _ ↔ (∀ j, ¬i ≺^[n + 1] j) ∧ (∃ j, i ≺^[n] j) := by simp [height_lt_iff_relItr, le_height_iff_relItr]
   _ ↔ (∀ k j, i ≺^[n] j → ¬j ≺ k) ∧ (∃ j, i ≺^[n] j) := by simp only [HRel.Iterate.forward, not_exists, not_and]
   _ ↔ (∃ j, i ≺^[n] j) ∧ (∀ j, i ≺^[n] j → ∀ k, ¬j ≺ k) := by grind
 
-lemma exists_rank_terminal (i : F) : ∃ j, i ≺^[Frame.World.finHeight i] j := le_finHeight_iff_relItr.mp (by simp)
+lemma exists_rank_terminal (i : F) : ∃ j, i ≺^[F.rank i] j := le_height_iff_relItr.mp (by simp)
 
-lemma eq_finHeight_root : Frame.World.finHeight x = F.finHeight ↔ x = r := by
+lemma eq_height_root : Frame.rank x = F.height ↔ x = r := by
   constructor;
   . rintro h;
     contrapose! h;
     apply Nat.ne_of_lt;
-    apply Frame.World.finHeight_lt_whole_finHeight;
+    apply Frame.rank_lt_whole_height;
     apply F.root_genaretes'!;
     assumption;
   . tauto;
 
-lemma terminal_rel_finHeight (h : x ≺^[World.finHeight x] y) : ∀ z, ¬y ≺ z := by
+lemma terminal_rel_height (h : x ≺^[rank x] y) : ∀ z, ¬y ≺ z := by
   intro z Ryz;
-  suffices World.finHeight x + 1 ≤ World.finHeight x by omega;
-  exact le_finHeight_iff_relItr.mpr ⟨z, HRel.Iterate.forward.mpr ⟨y, h, Ryz⟩⟩;
+  suffices rank x + 1 ≤ rank x by omega;
+  exact le_height_iff_relItr.mpr ⟨z, HRel.Iterate.forward.mpr ⟨y, h, Ryz⟩⟩;
 
 namespace extendRoot
 
-@[simp] lemma finHeight_pos : 0 < (F.extendRoot 1).finHeight := by
+@[simp] lemma height_pos : 0 < (F.extendRoot 1).height := by
   apply lt_fcwHeight ?_ (by simp)
   · exact Sum.inr r
   trivial
 
-@[simp] lemma finHeight₁ : (F.extendRoot 1).finHeight = F.finHeight + 1 := by
-  let l := World.finHeight (extendRoot.root : F.extendRoot 1)
+@[simp] lemma height_succ : (F.extendRoot 1).height = F.height + 1 := by
+  let l := rank (extendRoot.root : F.extendRoot 1)
   suffices
-      l ≤ Frame.World.finHeight r + 1 ∧
-      Frame.World.finHeight r < l by
+      l ≤ Frame.rank r + 1 ∧
+      Frame.rank r < l by
     simpa using Nat.eq_iff_le_and_ge.mpr this
   constructor
-  · suffices l - 1 ≤ World.finHeight r from Nat.le_add_of_sub_le this
-    apply le_finHeight_iff_relItr.mpr
+  · suffices l - 1 ≤ rank r from Nat.le_add_of_sub_le this
+    apply le_height_iff_relItr.mpr
     by_cases hl : l - 1 = 0
     · exact ⟨r, by simp [hl]⟩
     have lpos : 0 < l - 1 := Nat.zero_lt_of_ne_zero hl
     have e : l = (l - 1) + 1 := by
-      symm; exact Nat.sub_add_cancel Frame.extendRoot.finHeight_pos
+      symm; exact Nat.sub_add_cancel Frame.extendRoot.height_pos
     have : ∃ j, extendRoot.root ≺^[l] j := exists_rank_terminal (extendRoot.root : F.extendRoot 1)
     rcases this with ⟨j, hj⟩
     have : ∃ z, extendRoot.root ≺ z ∧ z ≺^[l - 1] j := by
       rw [e] at hj
       simpa using hj
     rcases this with ⟨z, hz, hzj⟩
-    have : ∃ x, j = embed x := eq_inr_of_root_rel <| HRel.Iterate.unwrap_of_trans_of_pos finHeight_pos hj
+    have : ∃ x, j = embed x := eq_inr_of_root_rel <| HRel.Iterate.unwrap_of_trans_of_pos height_pos hj
     rcases this with ⟨j, rfl⟩
     rcases not_root_of_from_root'₁ hz with (rfl | ⟨z, rfl, Rrz⟩)
     · exact ⟨j, embed_rel_iterate_embed_iff_rel.mp hzj⟩
     use j
     exact HRel.Iterate.constant_trans_of_pos lpos Rrz (embed_rel_iterate_embed_iff_rel.mp hzj)
-  · suffices World.finHeight r + 1 ≤ World.finHeight extendRoot.root from this
-    apply le_finHeight_iff_relItr.mpr
+  · suffices rank r + 1 ≤ rank extendRoot.root from this
+    apply le_height_iff_relItr.mpr
     rcases exists_rank_terminal r with ⟨j, hj⟩
     exact ⟨j, r, by trivial, embed_rel_iterate_embed_iff_rel.mpr hj⟩
 
-lemma eq_original_finHeight : Frame.World.finHeight (x : F.extendRoot 1) = Frame.World.finHeight x := by
-  apply finHeight_eq_iff_relItr.mpr;
+lemma eq_original_height : Frame.rank (x : F.extendRoot 1) = Frame.rank x := by
+  apply height_eq_iff_relItr.mpr;
   constructor;
   . obtain ⟨y, Rxy⟩ := exists_rank_terminal (i := x);
     use y;
@@ -133,24 +133,24 @@ lemma eq_original_finHeight : Frame.World.finHeight (x : F.extendRoot 1) = Frame
       exact Frame.irrefl _ this;
     . apply Frame.asymm;
       exact Frame.root_genaretes'! (F := F.extendRoot 1) y (by simp);
-    . have := terminal_rel_finHeight $ extendRoot.embed_rel_iterate_embed_iff_rel.mp Rxy;
+    . have := terminal_rel_height $ extendRoot.embed_rel_iterate_embed_iff_rel.mp Rxy;
       exact extendRoot.embed_rel_embed_iff_rel.not.mpr $ this z;
 
-lemma eq_original_finHeight_root : Frame.World.finHeight (r : F.extendRoot 1) = F.finHeight := eq_original_finHeight
+lemma eq_original_height_root : (F.extendRoot 1).rank r = F.height := eq_original_height
 
 @[grind]
-lemma iff_eq_finHeight_eq_original_root {x : F.extendRoot 1} : Frame.World.finHeight x = F.finHeight ↔ x = r := by
+lemma iff_eq_height_eq_original_root {x : F.extendRoot 1} : Frame.rank x = F.height ↔ x = r := by
   constructor;
   . rcases x with (a | x);
     . intro h;
-      have := h ▸ finHeight₁ (F := F);
-      simp [Frame.finHeight] at this;
+      have := h ▸ height_succ (F := F);
+      simp [Frame.height] at this;
     . intro h;
       suffices x = r by simp [this];
-      apply Frame.eq_finHeight_root.mp;
-      exact h ▸ Frame.extendRoot.eq_original_finHeight.symm;
+      apply Frame.eq_height_root.mp;
+      exact h ▸ Frame.extendRoot.eq_original_height.symm;
   . rintro rfl;
-    exact eq_original_finHeight_root;
+    exact eq_original_height_root;
 
 end extendRoot
 
@@ -162,7 +162,7 @@ instance [Fintype F] : Fintype (F↾x) := by apply Subtype.fintype;
 
 instance [F.IsTree r] : (F↾x).IsTree ⟨x, by tauto⟩ := by constructor;
 
-axiom eq_original_finHeight (hxy : y = x ∨ x ≺^+ y) : Frame.World.finHeight (F := F↾x) (⟨y, hxy⟩) = Frame.World.finHeight y
+axiom eq_original_height (hxy : y = x ∨ x ≺^+ y) : Frame.rank (F := F↾x) (⟨y, hxy⟩) = Frame.rank y
 
 end pointGenerate
 
@@ -173,18 +173,18 @@ section
 
 variable {M : Model} {r : M.World} [M.IsFiniteTree r] [Fintype M]
 
-lemma finHeight_lt_iff_satisfies_boxbot {i : M} :
-    Frame.World.finHeight i < n ↔ i ⊧ □^[n] ⊥ := by
-  simp only [Frame.finHeight_lt_iff_relItr, Formula.Kripke.Satisfies.multibox_def]
+lemma height_lt_iff_satisfies_boxbot {i : M} :
+    M.rank i < n ↔ i ⊧ □^[n] ⊥ := by
+  simp only [Frame.height_lt_iff_relItr, Formula.Kripke.Satisfies.multibox_def]
   simp
 
-lemma finHeight_pos_of_dia {i : M} (hA : i ⊧ ◇ A) : 0 < Frame.World.finHeight i := by
+lemma height_pos_of_dia {i : M} (hA : i ⊧ ◇ A) : 0 < M.rank i := by
   have : ∃ j, i ≺ j ∧ j ⊧ A := Formula.Kripke.Satisfies.dia_def.mp hA
   rcases this with ⟨j, hj, _⟩
   apply lt_fcwHeight hj (by simp)
 
-@[simp] lemma Model.extendRoot.finHeight₁ :
-    (M.extendRoot 1).finHeight = M.finHeight + 1 := Frame.extendRoot.finHeight₁
+@[simp]
+lemma Model.extendRoot.height₁ : (M.extendRoot 1).height = M.height + 1 := Frame.extendRoot.height_succ
 
 end
 
